pddl_validate_plan.sml
@@ -5,12 +5,12 @@ open PDDL
 
   (* To do: recursively transform abstract syntax trees while returning error messages *)
 
-  val IsabelleStringImplode = implode;
-  val IsabelleStringExplode = explode;
-  val SMLCharImplode = String.implode;
-  val SMLCharExplode = String.explode;
+  val IsabelleStringImplode = implode
+  val IsabelleStringExplode = explode
+  val SMLCharImplode = String.implode
+  val SMLCharExplode = String.explode
 
-  type isa_prim_type = char list;
+  type isa_prim_type = char list
 
   val stringToIsabelle = IsabelleStringExplode
   fun stringListToIsabelle ss = (map stringToIsabelle ss)
@@ -21,29 +21,24 @@ open PDDL
 
   fun pddlTermToIsabelleTerm (prob_decs: ast_problem_decs) (t: PDDL_TERM) =
     let
-      val f = (fn t => case t of
-        (OBJ_CONS_TERM oc) => 
-          let
-            val isa_n = stringToIsabelle (pddl_obj_name oc);
-            val isa_f = Function isa_n
-          in
-            if (is_obj_fun prob_decs isa_n)
-            then Fun isa_f
-            else Ent (Const (pddlObjConsToIsabelleObject oc))
-          end
-      | (VAR_TERM v) => Ent (Var (pddlVarToIsabelleVariable v))
+      fun f (t': PDDL_TERM) = case t' of
+        (VAR_TERM v) => Sym (Var (pddlVarToIsabelleVariable v))
+      | (FUN_TERM (n, [])) => (
+          if (is_obj_fun prob_decs (stringToIsabelle n))
+          then Fun (Function (stringToIsabelle n), [])
+          else Sym (Const (Object (stringToIsabelle n)))
+        )
       | (FUN_TERM (n, ts)) => Fun (Function (stringToIsabelle n), map f ts)
-      )
     in
       f t
     end
 
   fun mk_pair x y = (x,y)
-  fun snd (a, b) = b
-  fun fst (a, b) = a
-  fun map_pair (f1: 'a -> 'c) (f2: 'b -> 'd) (p: ('a * 'b)) : ('c * 'd)
-    = case p of (a, b) => (f1 a, f2 b)
-
+  fun snd (_, b) = b
+  fun fst (a, _) = a
+  fun map_pair (f1: 'a -> 'c) (f2: 'b -> 'd) ((a, b): ('a * 'b)) : ('c * 'd) = 
+    (f1 a, f2 b)
+    
   fun type_str_cat_fun (l: string list list) = (String.concatWith ", ") (map (String.concatWith ", ") l)
 
   fun flattenTypedList (l: ('a list * 'b) list): ('a * 'b) list =
@@ -69,10 +64,10 @@ open PDDL
             (fn t => case t of
               PDDL_PRIM_TYPE "object" => 
                 exit_fail "'object' cannot be a subtype"
-            | t => 
+            | _ => 
                 pddlPrimTypeToIsabellePrimType t)
         in
-          flatMapTypedList1 pddlPrimTypeToIsabellePrimType pddlTypeToIsabelleSuperType typesDef
+          flatMapTypedList1 pddlPrimTypeToIsabelleSubType pddlTypeToIsabelleSuperType typesDef
         end
     | _ => []
 
@@ -97,7 +92,7 @@ open PDDL
 
   fun pddlPredDeclToIsabelle (p: ATOMIC_FORM_SKEL) =
     let 
-      val (name, params) = p;
+      val (name, params) = p
     in  
       PredDecl (Predicate (stringToIsabelle name),
         flatMapTypedList (pddlTypeToIsabelleType o snd) params)
@@ -121,15 +116,21 @@ open PDDL
       SOME funs_def => 
       let
         val _ = map (fn (h, r) => case (h, r) of
-          (("total-cost", (x::xs)), _) => exit_fail "Reserved function 'total-cost' cannot take arguments"
+          (("total-cost", (_::_)), _) => exit_fail "Reserved function 'total-cost' cannot take arguments"
         | (("total-cost", _), Obj_Type _) => exit_fail "Reserved function 'total-cost' must return a number"
+        | _ => true
         )
-        val (obj_funs, num_funs) = (List.partition (fn (v, t) => t <> Num_Type) funs_def);
-        val fHead = map_pair (Function o stringToIsabelle) pddlTypedListToIsabelleSig;
-        val fObj = flatMapTypedList (fn (h, r) => 
-          case fHead h of
-           (f, args) => ObjFunDecl (f, args, pddlFunTypeToIsabelleType r));
-        val fNum = flatMapTypedList (NumFunDecl o fHead o fst);
+        val (obj_funs, num_funs) = List.partition (fn (_, t) => t <> Num_Type) funs_def
+        fun fHead xs = map_pair (Function o stringToIsabelle) pddlTypedListToIsabelleSig xs
+        fun fObj xs = 
+          flatMapTypedList (
+            fn (h, r) => 
+              let 
+                val (f, args) = fHead h;
+              in 
+                ObjFunDecl (f, args, pddlFunTypeToIsabelleType r)
+              end) xs
+        fun fNum xs = flatMapTypedList (NumFunDecl o fHead o fst) xs
       in 
         (fObj obj_funs, fNum num_funs)
       end
@@ -140,62 +141,80 @@ open PDDL
       SOME objs1  => flatMapTypedList1 pddlObjConsToIsabelleObject pddlTypeToIsabelleType objs1
     | NONE        => []
 
-  fun pddlAtomToIsabellePredicate (f: 'a -> 'b) (atom: 'a PDDL_ATOM) =
-    case atom of 
-      PDDL_Pred (name, ts) => Pred (Predicate (stringToIsabelle name), map f ts)
-    | PDDL_Pred_Eq (t1, t2)  => Eqa (f t1, f t2)
-
-  fun pddlTermAtomToIsabellePredicate (prob_decs: ast_problem_decs): PDDL_TERM PDDL_ATOM -> symbol term predicate = 
-    pddlAtomToIsabellePredicate (pddlTermToIsabelleTerm prob_decs)
-
 
   fun pddlFHeadToIsabelleFHead (prob_decs: ast_problem_decs) ((f, args): F_HEAD): (func * (symbol term list)) = 
     (Function (stringToIsabelle f), map (pddlTermToIsabelleTerm prob_decs) args)
 
+  fun pddlNFunHeadToIsabelleFHead (prob_decs: ast_problem_decs) (t: PDDL_TERM): (func * (symbol term list)) = 
+    case t of
+      (VAR_TERM _) => exit_fail "Numeric parameters (variables as function heads) not allowed"
+    | (FUN_TERM (f, args)) => (Function (stringToIsabelle f), map (pddlTermToIsabelleTerm prob_decs) args)
+
+  fun pddlNFunHeadToIsabelleNFun prob_decs = 
+    NFun o (pddlNFunHeadToIsabelleFHead prob_decs)
+
   fun pddlFExpToIsabelleNFluent (prob_decs: ast_problem_decs) (exp: PDDL_F_EXP) =
     let 
-      val f = (fn exp =>
-      case exp of
+      fun f e = case e of
         PDDL_Num (i, d) => Num (rat_from_strings (stringToIsabelle i) (Option.map stringToIsabelle d))
-      | F_Head h => NFun (pddlFHeadToIsabelleFHead prob_decs h)
-      | PDDL_Neg e => f (PDDL_Minus (PDDL_Num ("0", NONE), e))
+      | F_Head h => pddlNFunHeadToIsabelleNFun prob_decs h
+      | PDDL_Neg e' => f (PDDL_Minus (PDDL_Num ("0", NONE), e'))
       | PDDL_Minus (e1, e2) => Sub (f e1, f e2) 
       | PDDL_Div (e1, e2) => Div (f e1, f e2)
       | PDDL_Times es => mult_list (map f es)
       | PDDL_Plus es => add_list (map f es)
-      )
     in
       f exp
     end
 
-  (* Code duplication and potential error in disambiguation *)
-  fun pddlFHeadToIsabelleTerm (prob_decs: ast_problem_decs) ((f, args): F_HEAD): symbol term =
-    case (args) of
-      [] => pddlTermToIsabelleTerm(OBJ_CONS_TERM f)
-    | (x::xs) => pddlTermToIsabelleTerm(FUN_TERM (f, args))
-  
-  fun pddlFExpToIsabelleTerm (prob_decs: ast_problem_decs) (exp: PDDL_F_EXP) =
+  (* The FExp here can actually store variables and such *)
+  fun pddlFExpToIsabelleTerm (prob_decs: ast_problem_decs) (exp: PDDL_F_EXP): symbol term =
     case exp of 
-      F_Head h => NFun (pddlFHeadToIsabelleTerm prob_decs h)
+      F_Head h => pddlTermToIsabelleTerm prob_decs h
     | _ => exit_fail "Cannot assign number to object function."
 
-  fun pddlCompToIsabelleComp (prob_decs: ast_problem_decs) (comp: PDDL_F_COMP) =
-    case comp of
-      PDDL_Num_Lt (e1, e2) => Num_Lt (pddlFExpToIsabelleNFluent e1, pddlFExpToIsabelleNFluent e2)
-    | PDDL_Num_Le (e1, e2) => Num_Le (pddlFExpToIsabelleNFluent e1, pddlFExpToIsabelleNFluent e2)
-    | PDDL_Num_Eq (e1, e2) => Num_Eq (pddlFExpToIsabelleNFluent e1, pddlFExpToIsabelleNFluent e2)
-    | PDDL_Num_Gt (e1, e2) => Num_Le (pddlFExpToIsabelleNFluent e2, pddlFExpToIsabelleNFluent e1)
-    | PDDL_Num_Ge (e1, e2) => Num_Lt (pddlFExpToIsabelleNFluent e2, pddlFExpToIsabelleNFluent e1)
+  fun is_pddl_num_fun (prob_decs: ast_problem_decs) (t: PDDL_TERM): bool =
+    case t of 
+      (FUN_TERM (f, _)) => is_num_fun prob_decs (stringToIsabelle f)
+    | (VAR_TERM _) => false
+      
+
+  fun pddlEqToIsabelleEq (prob_decs: ast_problem_decs) (e1: PDDL_F_EXP) (e2: PDDL_F_EXP): symbol term atom =
+    let 
+      val to_num_fluent = pddlFExpToIsabelleNFluent prob_decs
+      val is_n = is_pddl_num_fun prob_decs
+    in
+      case (e1, e2) of 
+        (F_Head h1, F_Head h2) => (
+          case (is_n h1, is_n h2) of
+            (false, false) => PredAtom (Eqa (pddlTermToIsabelleTerm prob_decs h1, pddlTermToIsabelleTerm prob_decs h2))
+          | (true, true) => NumComp (Num_Eq (pddlNFunHeadToIsabelleNFun prob_decs h1, pddlNFunHeadToIsabelleNFun prob_decs h2))
+          | _ => exit_fail "Cannot compare numeric term to non-numeric term")
+      | _ => NumComp (Num_Eq (to_num_fluent e1, to_num_fluent e2))
+    end
+  
+  fun pddlTermAtomToIsabelleAtom (prob_decs: ast_problem_decs) (atom: PDDL_TERM_ATOM): symbol term atom = 
+    let 
+      val f = pddlFExpToIsabelleNFluent prob_decs
+    in
+      case atom of 
+        PDDL_Pred (name, ts) => PredAtom (Pred (Predicate (stringToIsabelle name), map (pddlTermToIsabelleTerm prob_decs) ts))
+      | PDDL_Eq (e1, e2) => pddlEqToIsabelleEq prob_decs e1 e2
+      | PDDL_Num_Lt (e1, e2) => NumComp (Num_Lt (f e1, f e2))
+      | PDDL_Num_Le (e1, e2) => NumComp (Num_Le (f e1, f e2))
+      | PDDL_Num_Gt (e1, e2) => NumComp (Num_Le (f e2, f e1))
+      | PDDL_Num_Ge (e1, e2) => NumComp (Num_Lt (f e2, f e1))
+    end
 
   val pddlVarParamsToIsabelleParams: (PDDL_VAR PDDL_TYPED_LIST) -> (PDDL_Checker_Exported.variable * typea) list =
-          flatMapTypedList1 pddlVarToIsabelleVariable pddlTypeToIsabelleType;
+          flatMapTypedList1 pddlVarToIsabelleVariable pddlTypeToIsabelleType
 
   fun pddlFormToIsabelleForm (prob_decs: ast_problem_decs) (phi: PDDL_FORM) =
       let 
-        fun f1 (phi: PDDL_FORM): symbol term atom formula = case phi of 
-          PDDL_Form_Atom atom   => Atom (PredAtom (pddlTermAtomToIsabellePredicate atom))
-        | PDDL_Form_Comp comp   => Atom (NumComp (pddlCompToIsabelleComp comp))
+        fun f1 (phi': PDDL_FORM): symbol term atom formula = case phi' of 
+          PDDL_Form_Atom atom   => Atom (pddlTermAtomToIsabelleAtom prob_decs atom)
         | PDDL_Not f            => Not (f1 f)
+        | PDDL_Imply (a, b)   => Imp (f1 a, f1 b)
         | PDDL_And fs           => bigAnd (map f1 fs)
         | PDDL_Or fs            => bigOr (map f1 fs)
         | PDDL_All (vts, f)     => pddl_all_impl prob_decs (pddlVarParamsToIsabelleParams vts) (f1 f)
@@ -221,8 +240,8 @@ open PDDL
     Left of 'a
   | Right of 'b
 
-  fun opAndFHeadAndExpToIsaNfUpd (oper: upd_op) (h: F_HEAD) (v: PDDL_F_EXP): symbol term nf_upd =
-    NF_Upd (flat43 (oper, flatl3 (pddlFHeadToIsabelleFHead h, pddlFExpToIsabelleNFluent v)))
+  fun opAndFHeadAndExpToIsaNfUpd (prob_decs: ast_problem_decs) (oper: upd_op) (h: F_HEAD) (v: PDDL_F_EXP): symbol term nf_upd =
+    NF_Upd (flat43 (oper, flatl3 (pddlFHeadToIsabelleFHead prob_decs h, pddlFExpToIsabelleNFluent prob_decs v)))
 
   (* 0-ary functions are indistinguishable from objects, which means we have to add the well-formedness condition
       that no 0-ary function has the same name as an object. Additionally, we implicitly rely on the parser to 
@@ -235,16 +254,20 @@ open PDDL
       *)
   fun pddlAssignToIsabelleUpd 
       (prob_decs: ast_problem_decs) (h: F_HEAD) 
-      (v: PDDL_TERM): symbol term ast_effect =
+      (v: PDDL_F_EXP): symbol term ast_effect =
     let
-      val (n, args) = h;
-      val isa_f = Function (stringToIsabelle n)
+      val isa_n = stringToIsabelle (fst h)
     in
-      case (is_obj_fun prob_decs isa_f, is_num_fun prob_decs isa_f) of
-        (True, _) => ofUpdToEff (OF_Upd (flatl3 (pddlFHeadToIsabelleFHead h, SOME (pddlFExpToIsabelleTerm v))))
-      | (_, True) => nfUpdToEff (opAndFHeadAndExpToIsaNfUpd Assign h v)
-      | _  => exit_fail ("Function '" ^ n ^ "' is undefined")
+      case (is_obj_fun prob_decs isa_n, is_num_fun prob_decs isa_n) of
+        (true, _) => ofUpdToEff (OF_Upd (flatl3 (pddlFHeadToIsabelleFHead prob_decs h, SOME (pddlFExpToIsabelleTerm prob_decs v))))
+      | (_, true) => nfUpdToEff (opAndFHeadAndExpToIsaNfUpd prob_decs Assign h v)
+      | _  => exit_fail ("Function '" ^ (fst h) ^ "' is undefined")
     end
+
+  fun pddlTermAtomToIsabellePredicate (prob_decs: ast_problem_decs) (a: PDDL_TERM_ATOM): symbol term predicate = 
+    case (pddlTermAtomToIsabelleAtom prob_decs a) of
+      PredAtom x => x
+    | _ => exit_fail "Not a predicate or object equality"
 
   fun pddlEffToIsabelleCondEffList 
       (prob_decs: ast_problem_decs) (eff: PDDL_EFFECT option): 
@@ -252,14 +275,14 @@ open PDDL
     let 
       fun f1 (eff: PDDL_EFFECT): symbol term ast_effect =
         (case eff of
-          Add p => Effect ([pddlTermAtomToIsabellePredicate p], [], [], [])
-        | Del p => Effect ([], [pddlTermAtomToIsabellePredicate p], [], [])
-        | Unassign h => ofUpdToEff (OF_Upd (flatl3 (pddlFHeadToIsabelleFHead h, NONE)))
+          Add p => Effect ([pddlTermAtomToIsabellePredicate prob_decs p], [], [], [])
+        | Del p => Effect ([], [pddlTermAtomToIsabellePredicate prob_decs p], [], [])
+        | Unassign h => ofUpdToEff (OF_Upd (flatl3 (pddlFHeadToIsabelleFHead prob_decs h, NONE)))
         | PDDL_Assign (h, v) => pddlAssignToIsabelleUpd prob_decs h v 
-        | N_ScaleUp (h, v) => nfUpdToEff (opAndFHeadAndExpToIsaNfUpd ScaleUp h v)
-        | N_ScaleDown (h, v) => nfUpdToEff (opAndFHeadAndExpToIsaNfUpd ScaleDown h v)
-        | N_Increase (h, v) => nfUpdToEff (opAndFHeadAndExpToIsaNfUpd Increase h v)
-        | N_Decrease (h, v) => nfUpdToEff (opAndFHeadAndExpToIsaNfUpd Decrease h v)
+        | N_ScaleUp (h, v) => nfUpdToEff (opAndFHeadAndExpToIsaNfUpd prob_decs ScaleUp h v)
+        | N_ScaleDown (h, v) => nfUpdToEff (opAndFHeadAndExpToIsaNfUpd prob_decs ScaleDown h v)
+        | N_Increase (h, v) => nfUpdToEff (opAndFHeadAndExpToIsaNfUpd prob_decs Increase h v)
+        | N_Decrease (h, v) => nfUpdToEff (opAndFHeadAndExpToIsaNfUpd prob_decs Decrease h v)
         | EFF_And _ => exit_fail "EFF_And does not result in a simple effect"
         | EFF_Cond _ => exit_fail "EFF_Cond does not result in a simple effect"
         | EFF_All _ => exit_fail "EFF_All does not result in a simpl_effect"
@@ -267,15 +290,15 @@ open PDDL
       and f2 (eff: PDDL_EFFECT): (symbol term atom formula * symbol term ast_effect) list =
         (case eff of
           EFF_And effs        => List.concat (map f2 effs)
-        | EFF_Cond (pre, eff) => 
+        | EFF_Cond (pre, e) => 
             map (fn (p, e) => 
               if (p = Not Bot)
               then (pddlFormToIsabelleForm prob_decs pre, e)
               else (And (p, pddlFormToIsabelleForm prob_decs pre), e)
-              ) (f2 eff)
-        | EFF_All (vts, eff)  => pddl_univ_effect_list_impl prob_decs (pddlVarParamsToIsabelleParams vts) (f2 eff)
-        | eff       => [(Not Bot, f1 eff)]
-        );
+              ) (f2 e)
+        | EFF_All (vts, e)  => pddl_univ_effect_list_impl prob_decs (pddlVarParamsToIsabelleParams vts) (f2 e)
+        | e       => [(Not Bot, f1 e)]
+        )
     in
       case eff of 
         SOME (eff: PDDL_EFFECT) => f2 eff
@@ -305,9 +328,11 @@ open PDDL
       (actsDef : PDDL_ACTION list) =
     map (pddlActToIsabelle prob_decs) actsDef
 
-  val pddlObjAtomToIsabelleObjPredicate: PDDL_OBJ_CONS PDDL_ATOM -> object predicate =
-    pddlAtomToIsabellePredicate pddlObjConsToIsabelleObject
-
+  fun pddlObjAtomToIsabelleObjPredicate (a: PDDL_OBJ_ATOM): object predicate =
+    case a of
+      PDDL_Obj_Pred (f, args) => Pred (Predicate (stringToIsabelle f), map pddlObjConsToIsabelleObject args)
+    | PDDL_Obj_Eq (o1, o2)    => Eqa (pddlObjConsToIsabelleObject o1, pddlObjConsToIsabelleObject o2)
+  
   fun pddlInitPredToIsabellePred
       (init: PDDL_INIT): object predicate list =
     case init of 
@@ -342,7 +367,7 @@ open PDDL
   fun initIsObjFunAsmt (init: PDDL_INIT) =
     case init of 
       Init_Obj_Func_Asmt _ => true
-    | _ => exit_fail "Invalid assignment to object function"
+    | _ => false
 
   fun initIsNumFunAsmt (init: PDDL_INIT) =
     case init of 
@@ -354,9 +379,9 @@ open PDDL
         (func * (object list * object)) list * (* Isabelle exported a weird product type *)
         (func * (object list * rat)) list =
     let 
-      val (preds, other) = List.partition initIsPredicate ls;
-      val (initO, initN) = List.partition initIsObjFunAsmt other;
-      val b = List.all initIsNumFunAsmt initN;
+      val (preds, other) = List.partition initIsPredicate ls
+      val (initO, initN) = List.partition initIsObjFunAsmt other
+      val _ = List.all initIsNumFunAsmt initN
     in
       (List.concat (map pddlInitPredToIsabellePred preds), 
         map (invflat3 o pddlInitObjFunAsmtToIsabelleObjFunAsmt) initO, 
@@ -371,9 +396,9 @@ open PDDL
         consts_def: PDDL_CONSTS_DEF option, 
         pred_def: PDDL_PREDS_DEF option, 
         funs_def: PDDL_FUNS_DEF option, 
-        actions_def: PDDL_ACTIONS_DEF): ast_domain_decs = 
+        _: PDDL_ACTIONS_DEF): ast_domain_decs = 
     let 
-      val (obj_funs, num_funs) = pddlFunsDefToIsabelleFuns funs_def;
+      val (obj_funs, num_funs) = pddlFunsDefToIsabelleFuns funs_def
     in
       PDDL_Checker_Exported.DomainDecls 
        (pddlTypesDefToIsabelle types_def,
@@ -394,10 +419,10 @@ open PDDL
   
   fun pddlDomAndProbDecsToIsaDom 
       (prob_decs: ast_problem_decs)
-      (types_def: PDDL_TYPES_DEF option, 
-        consts_def: PDDL_CONSTS_DEF option, 
-        pred_def: PDDL_PREDS_DEF option, 
-        funs_def: PDDL_FUNS_DEF option, 
+      (_: PDDL_TYPES_DEF option, 
+        _: PDDL_CONSTS_DEF option, 
+        _: PDDL_PREDS_DEF option, 
+        _: PDDL_FUNS_DEF option, 
         actions_def: PDDL_ACTIONS_DEF): ast_domain =
     PDDL_Checker_Exported.Domain
       (prob_decs, 
@@ -405,11 +430,11 @@ open PDDL
 
   fun pddlProbAndIsaDomToIsabelleProb 
       (dom: ast_domain)
-      (objs: PDDL_OBJ_DEF option,
+      (_: PDDL_OBJ_DEF option,
         init: PDDL_INIT list,
         goal_form: PDDL_GOAL): ast_problem = 
     case dom of 
-      PDDL_Checker_Exported.Domain (prob_decs, actions) => 
+      PDDL_Checker_Exported.Domain (prob_decs, _) => 
         PDDL_Checker_Exported.Problem(
           flat535 (dom, pddlInitListToIsabelleInit init, 
           pddlGoalToIsabelle prob_decs goal_form))
@@ -443,13 +468,13 @@ val parse_pddl_plan = parse_wrapper PDDL.plan
 
 
 fun do_check_plan dom_file prob_file plan_file = let
-  val _ = println "here";
+
   val parsedDom = parse_pddl_dom dom_file
-  val _ = println "1";
+
   val parsedProb = parse_pddl_prob prob_file
-  val _ = println "2";
+
   val parsedPlan = parse_pddl_plan plan_file
-  val _ = println "3";
+
   val isaDomDecs = pddlDomToIsabelleDomDecs parsedDom
   val isaProbDecs = pddlProbAndDomDecsToIsaProbDecs isaDomDecs parsedProb
   val isaDom = pddlDomAndProbDecsToIsaDom isaProbDecs parsedDom
@@ -471,19 +496,19 @@ fun print_help () = (
   println("c Usage: " ^ CommandLine.name() ^ "<domain> <problem> [<plan>]")
 )
 val _ = case args of
-  ("--test"::(f::xs)) => 
+  ("--test"::(f::_)) => 
     let 
       val _ = println ("parsing: " ^ f)
-      val parse_effect = parse_wrapper PDDL.effect
-      val _ = parse_effect f
+      val parser = parse_wrapper PDDL.pre_GD
+      val _ = parser f
     in
       println "here"
     end
 | [d,pr,pl] => do_check_plan d pr pl
 | _ => (
-    println("Invalid command line arguments");
-    print_help ();
+    println "Invalid command line arguments";
+    print_help;
     exit_fail ""
   )
 
-val _ = OS.Process.exit(OS.Process.success)
+val _ = OS.Process.exit OS.Process.success
